examples/lrat_checker/lratScript.sml
@@ -7,34 +7,41 @@ val _ = new_theory "lrat";
 
 (*** Semantics ***
 
-  For now, the semantics is rather low level
-  It would be worth defining a more abstract notion of this that doesn't mess
-  concretely with -1,1 etc.
+  A literal is drawn from the sum 'a + 'a with the left projection being positive
+  and the right projection being negative
 
-  A clause is a list of literals (ints)
-  A CNF is a set of clauses
+  A clause is a set of literals (understood disjunctively)
 
-  An assignment is a map from the natural numbers (including 0) to T/F
+  A CNF is a set of clauses (understood conjunctively)
+
+  An assignment is a map from 'a to T/F
 
   A clause is satisfied by an assignment if there is at least one of its literals assigned to true
   A CNF is satisfied by an assignment if all its clauses are satisfied
 *)
 
-Type clause = ``:int list``;
-Type cnf = ``:clause set``;
-Type assignment = ``:num -> bool``;
+Type clause = ``:('a + 'a) set``;
+Type cnf = ``:'a clause set``;
+Type assignment = ``:'a -> bool``;
+
+val negate_literal_def = Define`
+  negate_literal l=
+  case l of
+    INL x => INR x
+  | INR x => INL x`
 
 val satisfies_literal_def = Define`
-  satisfies_literal (w:assignment) l ⇔
-  if l ≥ 0 then w (Num (ABS l))
-  else ~w (Num (ABS l))`
+  satisfies_literal (w:'a assignment) l ⇔
+  case l of
+    INL x => w x
+  | INR x => ¬w x`
 
 val satisfies_clause_def = Define`
-  satisfies_clause (w:assignment) (C:clause) ⇔
-  ∃l. MEM l C ∧ satisfies_literal w l`
+  satisfies_clause (w:'a assignment) (C:'a clause) ⇔
+  ∃l. l ∈ C ∧ satisfies_literal w l`
 
 val satisfies_def = Define`
-  satisfies (w:assignment) (fml:cnf) ⇔
+  satisfies (w:'a assignment) (fml:'a cnf) ⇔
   ∀C. C ∈ fml ⇒ satisfies_clause w C`
 
 val satisfiable_def = Define`
@@ -49,24 +56,30 @@ val unsatisfiable_def = Define`
 
 (* Empty clauses are unsat *)
 Theorem empty_clause_imp_unsatisfiable:
-  [] ∈ fml ⇒
+  {} ∈ fml ⇒
   unsatisfiable fml
 Proof
   rw[unsatisfiable_def,satisfiable_def,satisfies_def,satisfies_clause_def]>>
-  qexists_tac`[]`>> simp[]
+  asm_exists_tac>>fs[]
+QED
+
+Theorem negate_negate[simp]:
+  negate_literal(negate_literal l) = l
+Proof
+  Cases_on`l`>>fs[negate_literal_def]
 QED
 
 (* l , -l are duals *)
 Theorem satisfies_literal_exclusive:
-  l ≠ 0 ⇒
-  (satisfies_literal w l ⇔  ¬satisfies_literal w (-l))
+  (satisfies_literal w l ⇔  ¬satisfies_literal w (negate_literal l))
 Proof
   rw[EQ_IMP_THM,satisfies_literal_def]>>
-  fs[] >> `F` by intLib.ARITH_TAC
+  every_case_tac>>fs[negate_literal_def]>>
+  rfs[]
 QED
 
 Theorem unsat_negate_satisfies_literal:
-  l ≠ 0 ∧ unsatisfiable ([-l] INSERT fml) ∧
+  unsatisfiable ({negate_literal l} INSERT fml) ∧
   satisfies w fml ⇒
   satisfies_literal w l
 Proof
@@ -79,6 +92,14 @@ Proof
   >>
     metis_tac[]
 QED
+
+Theorem satisfies_clause_INSERT:
+  satisfies_clause w (l INSERT C) ⇔ satisfies_literal w l ∨ satisfies_clause w C
+Proof
+  rw[satisfies_clause_def]>>
+  metis_tac[]
+QED
+
 
 Theorem satisfies_INSERT:
   satisfies w (C INSERT fml) ⇔ satisfies_clause w C ∧ satisfies w fml
@@ -119,7 +140,7 @@ Proof
 QED
 
 Theorem sing_satisfies_literal:
-  [l] ∈ fml ∧
+  {l} ∈ fml ∧
   satisfies w fml ⇒
   satisfies_literal w l
 Proof
@@ -129,18 +150,18 @@ Proof
 QED
 
 Theorem satisfies_clause_append:
-  satisfies_clause w (A++B) ⇔ satisfies_clause w A ∨ satisfies_clause w B
+  satisfies_clause w (A ∪ B) ⇔ satisfies_clause w A ∨ satisfies_clause w B
 Proof
   fs[satisfies_clause_def]>>
   metis_tac[]
 QED
 
 Theorem satisfies_clause_SUBSET:
-  (∀l. MEM l (C:clause) ⇒ MEM l C') ⇒
+  C ⊆ C' ∧
   satisfies_clause w C ⇒ satisfies_clause w C'
 Proof
   rw[satisfies_clause_def]>>
-  metis_tac[]
+  metis_tac[SUBSET_DEF]
 QED
 
 Theorem UNION_INSERT_EQ:
@@ -149,26 +170,21 @@ Proof
   fs[EXTENSION]>>metis_tac[]
 QED
 
-val wf_clause_def = Define`
-  wf_clause (C:clause) ⇔ ¬MEM 0 C`
-
 (* Definition of asymmetric tautologies *)
 val asymmetric_tautology_def = Define`
   asymmetric_tautology fml C ⇔
-  wf_clause C ∧
-  unsatisfiable (fml ∪ set (MAP (λl. [-l]) C))`
+  unsatisfiable (fml ∪ (IMAGE (λl. {negate_literal l}) C))`
 
 Theorem list_unsat_negate_satisfies_literal:
   ∀ls.
-  wf_clause ls ∧
-  unsatisfiable (fml ∪ set (MAP (λl. [-l]) ls)) ∧
+  unsatisfiable (fml ∪ (IMAGE (λl. {negate_literal l}) C)) ∧
   satisfies w fml ⇒
-  satisfies_clause w ls
+  satisfies_clause w C
 Proof
-  rw[unsatisfiable_def,satisfiable_def,satisfies_union,wf_clause_def]>>
+  rw[unsatisfiable_def,satisfiable_def,satisfies_union]>>
   first_x_assum(qspec_then`w` assume_tac)>>
   rfs[]>>
-  fs[satisfies_def,MEM_MAP]>>rw[]>>fs[satisfies_clause_def]>>
+  fs[satisfies_def]>>rw[]>>fs[satisfies_clause_def]>>
   metis_tac[satisfies_literal_exclusive]
 QED
 
@@ -210,53 +226,57 @@ Proof
 QED
 
 Theorem tautology_asymmetric_tautology:
-  wf_clause C ∧
-  MEM l C ∧ MEM (-l) C
+  l ∈ C ∧ negate_literal l ∈ C
   ⇒
   asymmetric_tautology fml C
 Proof
   rw[asymmetric_tautology_def,unsatisfiable_def,satisfiable_def,satisfies_def,MEM_MAP]>>
-  `l ≠ 0` by metis_tac[wf_clause_def]>>
   Cases_on`satisfies_literal w l`
   >-
-    (qexists_tac`[-l]`>>fs[satisfies_clause_def]>>
+    (qexists_tac`{negate_literal l}`>>fs[satisfies_clause_def]>>
     metis_tac[satisfies_literal_exclusive])
   >>
-    qexists_tac`[l]`>>fs[satisfies_clause_def]>>
+    qexists_tac`{l}`>>fs[satisfies_clause_def]>>
     DISJ2_TAC>>
-    qexists_tac`-l`>>simp[]
+    qexists_tac`negate_literal l`>>simp[]
 QED
 
-(* TODO: NOT efficient *)
 val delete_literal_def = Define`
-  delete_literal l (C:clause) =
-    FILTER (λi. i  <> l) C `
+  delete_literal l (C:'a clause) = C DIFF {l}`
+
+Theorem delete_literal_preserves_satisfies_clause_imp:
+  satisfies_clause w (delete_literal (negate_literal l) C) ⇒
+  satisfies_clause w C
+Proof
+  fs[delete_literal_def,satisfies_clause_def]>>
+  metis_tac[]
+QED
 
 Theorem delete_literal_preserves_satisfies_clause:
-  l ≠ 0 ∧ satisfies_literal w l ⇒
-  (satisfies_clause w C ⇔ satisfies_clause w (delete_literal (-l) C))
+  satisfies_literal w l ⇒
+  (satisfies_clause w C ⇔ satisfies_clause w (delete_literal (negate_literal l) C))
 Proof
   rw[EQ_IMP_THM]
   >- (
-    fs[delete_literal_def,satisfies_clause_def,MEM_FILTER]>>
+    fs[delete_literal_def,satisfies_clause_def]>>
     metis_tac[satisfies_literal_exclusive]
   )
   >>
-    fs[delete_literal_def,satisfies_clause_def,MEM_FILTER]>>
+    fs[delete_literal_def,satisfies_clause_def]>>
     metis_tac[]
 QED
 
 Theorem delete_unit_preserves_satisfies:
-  l ≠ 0 ∧ [l] ∈ fml ⇒
-  (satisfies w (C INSERT fml) ⇔ satisfies w ((delete_literal (-l) C) INSERT fml))
+  {l} ∈ fml ⇒
+  (satisfies w (C INSERT fml) ⇔ satisfies w ((delete_literal (negate_literal l) C) INSERT fml))
 Proof
   fs[satisfies_INSERT]>>
   metis_tac[delete_literal_preserves_satisfies_clause,sing_satisfies_literal]
 QED
 
 Theorem delete_unit_preserves_satisfiable:
-  l ≠ 0 ∧ [l] ∈ fml ⇒
-  (satisfiable (C INSERT fml) ⇔ satisfiable ((delete_literal (-l) C) INSERT fml))
+  {l} ∈ fml ⇒
+  (satisfiable (C INSERT fml) ⇔ satisfiable ((delete_literal (negate_literal l) C) INSERT fml))
 Proof
   fs[satisfiable_def]>>
   metis_tac[delete_unit_preserves_satisfies]
@@ -265,13 +285,13 @@ QED
 (* Definition of resolution asymmetric tautology *)
 val resolution_asymmetric_tautology_def = Define`
   resolution_asymmetric_tautology fml C ⇔
-  ¬MEM 0 C ∧
   (asymmetric_tautology fml C ∨
-  ∃l. MEM l C ∧
-  ∀D. D ∈ fml ∧ MEM (-l) D ⇒
-    asymmetric_tautology fml (C ++ delete_literal (-l) D))`
+  ∃l. l ∈ C ∧
+  ∀D. D ∈ fml ∧ negate_literal l ∈ D ⇒
+    asymmetric_tautology fml (C ∪ delete_literal (negate_literal l) D))`
 
 (* soundness of resolution step *)
+(*
 Theorem resolution_sound:
   l ≠ 0 ∧ (l::xs) ∈ fml ∧ ((-l)::ys) ∈ fml ⇒
   (satisfies w fml ⇔ satisfies w ((xs++ys) INSERT fml))
@@ -306,35 +326,39 @@ Proof
     match_mp_tac satisfies_SUBSET>>
     fs[SUBSET_DEF]
 QED
+*)
 
 val flip_literal_def = Define`
-  flip_literal l (w:assignment) =
-  λv. if v = Num (ABS l) then ¬w (Num (ABS l)) else w v`
+  flip_literal l (w:'a assignment) =
+  case l of
+    INL x =>
+    λv. if v = x then ¬w x else w v
+  | INR x =>
+    λv. if v = x then ¬w x else w v`
 
 Theorem flip_literal_eq_neg:
-  flip_literal l w = flip_literal (-l) w
+  flip_literal l w = flip_literal (negate_literal l) w
 Proof
-  simp[flip_literal_def]
+  simp[flip_literal_def]>>
+  TOP_CASE_TAC>>fs[negate_literal_def]
 QED
 
 Theorem flip_literal_flips:
-  l ≠ 0 ⇒
   (satisfies_literal w l ⇔ ¬(satisfies_literal (flip_literal l w) l))
 Proof
-  rw[satisfies_literal_def,flip_literal_def]
+  rw[satisfies_literal_def,flip_literal_def]>>
+  TOP_CASE_TAC>>fs[]
 QED
 
 Theorem flip_literal_unaffected:
-  l ≠ 0 ∧
   satisfies_literal w l ∧
-  satisfies_clause w C ∧ ¬ MEM l C ⇒
+  satisfies_clause w C ∧ l ∉ C ⇒
   satisfies_clause (flip_literal l w ) C
 Proof
   rw[satisfies_clause_def,satisfies_literal_def]>>
   asm_exists_tac>>fs[]>>rw[]>>fs[]>>
-  fs[flip_literal_def]>>
-  `l ≠ l'` by metis_tac[]>>
-  intLib.ARITH_TAC
+  every_case_tac>>fs[flip_literal_def]>>
+  metis_tac[]
 QED
 
 Theorem resolution_asymmetric_tautology_satisfiable:
@@ -351,7 +375,7 @@ Proof
   Cases_on`satisfies_clause w C`
   >-
     metis_tac[satisfies_INSERT]>>
-  qabbrev_tac`Ds = IMAGE (λD. C ++ delete_literal (-l) D) { D | D ∈ fml∧  MEM (-l) D}`>>
+  qabbrev_tac`Ds = IMAGE (λD. C ∪ delete_literal (negate_literal l) D) { D | D ∈ fml ∧  (negate_literal l) ∈  D}`>>
   `∀D. D ∈ Ds ⇒ asymmetric_tautology fml D` by
     (rw[]>>fs[Abbr`Ds`])>>
   drule asymmetric_tautology_set_satisfies >>
@@ -359,15 +383,14 @@ Proof
   strip_tac>>
   fs[satisfies_union]>>
   qabbrev_tac`w' = flip_literal l w`>>
-  qexists_tac`w'` >> rw[satisfies_INSERT]>>
-  `l ≠ 0` by metis_tac[]
+  qexists_tac`w'` >> rw[satisfies_INSERT]
   >- (
     `satisfies_literal w' l` by
       (simp[Abbr`w'`]>>
       metis_tac[flip_literal_flips,satisfies_clause_def])>>
     metis_tac[satisfies_clause_def])
   >>
-    `fml = { D | D ∈ fml ∧ ¬MEM (-l) D} ∪ { D | D ∈ fml ∧ MEM (-l) D}` by
+    `fml = { D | D ∈ fml ∧ ¬(negate_literal l ∈  D)} ∪ { D | D ∈ fml ∧ (negate_literal l ∈  D)}` by
       (simp[EXTENSION]>>
       metis_tac[])>>
     pop_assum SUBST1_TAC>>
@@ -376,55 +399,36 @@ Proof
       fs[satisfies_def]>>rw[]>>
       fs[Abbr`w'`]>>
       simp[Once flip_literal_eq_neg]>>
-      `-l ≠ 0` by fs[]>>
-      drule flip_literal_unaffected>>
-      disch_then match_mp_tac>> simp[]>>
+      match_mp_tac flip_literal_unaffected>>
       metis_tac[satisfies_literal_exclusive,satisfies_clause_def])
     >>
       fs[satisfies_def]>>rw[]>>
-      `C ++ delete_literal (-l) C' ∈ Ds` by
+      `C ∪ delete_literal (negate_literal l) C' ∈ Ds` by
         (fs[Abbr`Ds`]>>
         qexists_tac`C'`>>fs[])>>
       first_x_assum drule>> disch_then kall_tac>>
       first_x_assum drule>>
       simp[satisfies_clause_append]>>
       strip_tac>>
-      `satisfies_clause w' (delete_literal (-l) C')` by
+      `satisfies_clause w' (delete_literal (negate_literal l) C')` by
         (simp[Abbr`w'`]>>
         simp[Once flip_literal_eq_neg]>>
-        `-l ≠ 0` by fs[]>>
-        drule flip_literal_unaffected>>
-        disch_then match_mp_tac>>
-        fs[delete_literal_def,MEM_FILTER]>>
+        match_mp_tac flip_literal_unaffected>>
+        fs[delete_literal_def]>>
         metis_tac[satisfies_literal_exclusive,satisfies_clause_def])>>
-      pop_assum mp_tac>>
-      match_mp_tac satisfies_clause_SUBSET>>
-      fs[delete_literal_def,MEM_FILTER]
+      metis_tac[delete_literal_preserves_satisfies_clause_imp]
 QED
 
-(* More implementationy stuff *)
+(* Bridging implementation and semantics
+
+  Clauses are represented by two sptree sets
+  The left set corresponds to the "INL" and right to INR
+*)
+Type cclause = ``:num_set # num_set``;
+Type ccnf = ``:cclause spt``;
 
 val values_def = Define`
   values s = {v | ∃n. lookup n s = SOME v}`
-
-val wf_fml_def = Define`
-  wf_fml fml ⇔ ∀C. C ∈ values fml ⇒ wf_clause C`
-
-Theorem filter_unit_preserves_unsatisfiable:
-  ∀C.
-  wf_clause (C:clause) ∧
-  set (MAP (λl. [-l]) C) ⊆ fml ⇒
-  (unsatisfiable (D INSERT fml) ⇔ unsatisfiable ((FILTER (λx. ¬MEM x C) D) INSERT fml))
-Proof
-  Induct>>rw[]>>
-  fs[wf_clause_def]>>
-  simp[GSYM FILTER_FILTER,GSYM delete_literal_def]>>
-  `-h ≠ 0` by fs[]>>
-  drule delete_unit_preserves_satisfiable>>
-  disch_then drule>>
-  simp[]>>
-  metis_tac[unsatisfiable_def]
-QED
 
 Theorem values_delete:
   values (delete h v) ⊆ values v
@@ -449,23 +453,43 @@ Proof
   metis_tac[values_insert]
 QED
 
+val interp_cclause_def = Define`
+  interp_cclause ((L,R):cclause) =
+  IMAGE INL (domain L) ∪
+  IMAGE INR (domain R)`
+
+val interp_def = Define`
+  interp (fml:ccnf) = IMAGE interp_cclause (values fml)`
+
 (*** Implementation ***)
 val _ = Datatype`
   lratstep =
     Delete (num list) (* Clauses to delete *)
-  | RAT num clause (num list) ((num list) spt)`
+  | RAT num (num + num) cclause (num list) ((num list) spt)`
     (* RAT step:
-      AT n C i0 (ik id ~> ik)
+      RAT n p C i0 (ik id ~> ik)
       n is the new id of the new clause C
+      p is the pivot (first element of C in the input)
       i0 is a list of clause IDs for the AT part
       ik is a sptree mapping clause IDs to their hints
     *)
 
 Type lrat = ``:lratstep list``
 
-val delete_clauses_def = Define`
-  delete_clauses cl fml =
-    FOLDR delete fml cl`
+val list_delete_def = Define`
+  list_delete cl fml = FOLDR delete fml cl`
+
+(* C - D *)
+val delete_literals_def = Define`
+  delete_literals (C:cclause) (D:cclause) =
+  let dl = (MAP FST (toAList (FST D))) in
+  let dr = (MAP FST (toAList (SND D))) in
+  (list_delete dl (FST C), list_delete dr (SND C))`
+
+val insert_literal_def = Define`
+  insert_literal l b C =
+  if b then (insert l () (FST C),SND C)
+  else (FST C, insert l () (SND C))`
 
 (*
   Checking for asymmetric tautology via unit propagation using the given hints
@@ -474,25 +498,49 @@ val delete_clauses_def = Define`
   SOME (INR C) == hints were insufficient, but C is now extended with units
 *)
 val is_AT_def = Define`
-  (is_AT fml [] (C:clause) = SOME (INR C)) ∧
+  (is_AT fml [] (C:cclause) = SOME (INR C)) ∧
   (is_AT fml (i::is) C =
   case lookup i fml of
     NONE => NONE
   | SOME Ci =>
-  let D = FILTER (λx. ¬ MEM x C) Ci in
-  case D of
-    [] => SOME (INL ())
-  | [d] => is_AT fml is (-d::C)
+  let (Dl,Dr) = delete_literals Ci C in
+  let Dll = toAList Dl in
+  let Drr = toAList Dr in
+  case (Dll,Drr) of
+    ([],[])  => SOME (INL ())
+  | ([l,_],[]) => is_AT fml is (insert_literal l F C)
+  | ([],[l,_]) => is_AT fml is (insert_literal l T C)
   | _ => NONE)`
 
+val has_literal_def = Define`
+  has_literal l C =
+  case l of
+    INL x => lookup x (FST C) = SOME ()
+  | INR x => lookup x (SND C) = SOME ()`
+
+val has_neg_literal_def = Define`
+  has_neg_literal l C =
+  case l of
+    INL x => lookup x (SND C) = SOME ()
+  | INR x => lookup x (FST C) = SOME ()`
+
+val delete_neg_literal_def = Define`
+  delete_neg_literal l C =
+  case l of
+    INL x => (FST C, delete x (SND C))
+  | INR x => (delete x (FST C), SND C)`
+
+val find_exists_def = Define`
+  (find_exists s [] = F) ∧
+  (find_exists s (x::xs) = (lookup (FST x) s = SOME () ∨ find_exists s xs))`
+
 val find_tauto_def = Define`
-  (find_tauto p C [] = F) ∧
-  (find_tauto (p:int) C (c::cs) =
-    if c = -p then find_tauto p C cs
-    else
-      if MEM (-c) C then T
-      else find_tauto p C cs
-  )`
+  find_tauto (LC,RC) (LD,RD) =
+  (find_exists LC (toAList RD) ∨ find_exists RC (toAList LD))`
+
+val cclause_union_def = Define`
+  cclause_union (L1,R1) (L2,R2) =
+  (union L1 L2, union R1 R2)`
 
 (*
   Resolution Asymmetric Tautology
@@ -501,38 +549,37 @@ val is_RAT_aux_def = Define`
   (is_RAT_aux fml p C ik [] = T) ∧
   (is_RAT_aux fml p C ik (iCi::iCs) =
   case iCi of (i,Ci) =>
-    if MEM (-p) Ci then
+    if has_neg_literal p  Ci then
       case lookup i ik of
         NONE => F
       | SOME is =>
         case is of [] =>
         (* Step 5.2: can be made more efficient *)
-          if find_tauto p C Ci then
+          if find_tauto C (delete_neg_literal p Ci) then
             is_RAT_aux fml p C ik iCs
           else
             F
         | _ =>
-        (* Step 5.3-5.5 *)
-        if is_AT fml is (C ++ delete_literal (-p) Ci) = SOME (INL ()) then
-          is_RAT_aux fml p C ik iCs
-        else
-          F
+          (* Step 5.3-5.5 *)
+          if is_AT fml is (cclause_union C (delete_neg_literal p Ci)) = SOME (INL ()) then
+            is_RAT_aux fml p C ik iCs
+          else
+            F
     else
       is_RAT_aux fml p C ik iCs)`
 
 val is_RAT_def = Define`
-  is_RAT fml (C:clause) i0 ik =
+  is_RAT fml p (C:cclause) i0 ik =
   (* First, do the asymmetric tautology check *)
   case is_AT fml i0 C of
     NONE => F
   | SOME (INL ()) => T
   | SOME (INR D) =>
-  (* First, do the asymmetric tautology check *)
-  case C of
-    [] => F
-  | (p::C) =>
-  let iCs = toAList fml in
-    is_RAT_aux fml p D ik iCs`
+  if has_literal p C then
+    let iCs = toAList fml in
+      is_RAT_aux fml p D ik iCs
+  else
+     F`
 
 (* Run the LRAT checker on fml, returning an option *)
 val check_lrat_def = Define`
@@ -540,12 +587,10 @@ val check_lrat_def = Define`
   (check_lrat (step::steps) fml =
     case step of
       Delete cl =>
-      check_lrat steps (delete_clauses cl fml)
-    | RAT n C i0 ik =>
-      if wf_clause C then
-      if is_RAT fml C i0 ik then
+      check_lrat steps (list_delete cl fml)
+    | RAT n p C i0 ik =>
+      if is_RAT fml p C i0 ik then
         check_lrat steps (insert n C fml)
-      else NONE
       else NONE)`
 
 val check_lrat_unsat_def = Define`
@@ -554,150 +599,314 @@ val check_lrat_unsat_def = Define`
     NONE => F
   | SOME fml' =>
     let ls = MAP SND (toAList fml') in
-    MEM [] ls`
+    MEM (LN,LN) ls`
+
+Theorem filter_unit_preserves_satisfies:
+  ∀C.
+  (IMAGE (λl. {negate_literal l}) C) ⊆ fml ∧
+  satisfies w (D INSERT fml) ⇒
+  satisfies w ( (D DIFF C) INSERT fml)
+Proof
+  rw[satisfies_def]
+  >-
+    (first_assum(qspec_then`D` assume_tac)>>fs[satisfies_clause_def]>>
+    `l ∉ C` by
+      (CCONTR_TAC>>
+      fs[SUBSET_DEF]>>
+      last_x_assum(qspec_then`{negate_literal l}` mp_tac)>>
+      impl_tac >-
+        metis_tac[]>>
+      strip_tac>>
+      first_x_assum(qspec_then`{negate_literal l}` assume_tac)>>rfs[]>>
+      metis_tac[satisfies_literal_exclusive])>>
+    metis_tac[])
+  >>
+    metis_tac[]
+QED
+
+Theorem filter_unit_preserves_unsatisfiable:
+  ∀C.
+  (IMAGE (λl. {negate_literal l}) C) ⊆ fml ∧
+  unsatisfiable ((D DIFF C) INSERT fml) ⇒
+  unsatisfiable (D INSERT fml)
+Proof
+  rw[unsatisfiable_def,satisfiable_def]>>
+  metis_tac[filter_unit_preserves_satisfies]
+QED
+
+(*
+val wf_clause_def = Define`
+  wf_clause (C:cclause) ⇔
+  lookup cmp 0 C = NONE ∧
+  map_ok C`
+
+val wf_fml_def = Define`
+  wf_fml (f:ccnf) ⇔ ∀C. C ∈ values f ⇒ wf_clause C`
+*)
+
+Theorem list_delete_correct:
+  ∀ls sp x v.
+  lookup x (list_delete ls sp) = SOME v ⇔
+  lookup x sp = SOME v ∧ ¬MEM x ls
+Proof
+  Induct>>fs[list_delete_def,lookup_delete]>>
+  metis_tac[]
+QED
+
+Theorem list_delete_domain:
+  domain (list_delete ls sp) =
+  domain sp DIFF set ls
+Proof
+  rw[EXTENSION,domain_lookup]>>
+  metis_tac[list_delete_correct]
+QED
+
+Theorem delete_literals_correct:
+  interp_cclause (delete_literals C D) =
+  interp_cclause C DIFF interp_cclause D
+Proof
+  Cases_on`C`>>Cases_on`D`>>
+  simp[delete_literals_def]>>
+  fs[interp_cclause_def,list_delete_domain]>>
+  fs[EXTENSION,toAList_domain]>>
+  rw[EQ_IMP_THM]>>
+  metis_tac[]
+QED
+
+Theorem interp_cclause_toAList:
+  interp_cclause (L,R) =
+  set (MAP (INL o FST) (toAList L)) ∪
+  set (MAP (INR o FST) (toAList R))
+Proof
+  rw[interp_cclause_def,EXTENSION,GSYM MAP_MAP_o]>>
+  simp[Once MEM_MAP,toAList_domain]>>
+  simp[Once MEM_MAP,toAList_domain]
+QED
+
+Theorem interp_cclause_insert_literal:
+  (interp_cclause (insert_literal q T C) = INL q INSERT interp_cclause C) ∧
+  (interp_cclause (insert_literal q F C) = INR q INSERT interp_cclause C)
+Proof
+  Cases_on`C`>>rw[interp_cclause_def,insert_literal_def,EXTENSION]>>
+  metis_tac[]
+QED
 
 (* Implementation *)
 Theorem is_AT_imp_asymmetric_tautology:
   ∀is fml C.
-  wf_fml fml ∧ wf_clause C ∧
+  (* wf_fml fml ∧ wf_clause C ∧ *)
   is_AT fml is C = SOME (INL ()) ⇒
-  asymmetric_tautology (values fml) C
+  asymmetric_tautology (interp fml) (interp_cclause C)
 Proof
   Induct>>fs[is_AT_def]>>
   ntac 4 strip_tac>>
-  drule filter_unit_preserves_unsatisfiable>>
+  every_case_tac>>fs[]>>
+  pairarg_tac>>fs[]>>
+  `interp_cclause x DIFF interp_cclause C = interp_cclause (Dl,Dr)` by
+    metis_tac[delete_literals_correct]>>
   every_case_tac>>fs[]
   >-
     (fs[asymmetric_tautology_def]>>
-    rw[]>>
     qmatch_goalsub_abbrev_tac`unsatisfiable fml'`>>
-    `fml' = x INSERT fml'` by
+    `fml' = (interp_cclause x) INSERT fml'` by
       (match_mp_tac (GSYM ABSORPTION_RWT)>>
-      fs[Abbr`fml'`,values_def]>>
+      fs[Abbr`fml'`,values_def,interp_def]>>
       metis_tac[])>>
     pop_assum SUBST1_TAC>>
-    first_x_assum(qspecl_then[`fml'`,`x`] mp_tac)>>
-    impl_tac
+    match_mp_tac filter_unit_preserves_unsatisfiable>>
+    qexists_tac`interp_cclause C`>>rw[]
     >-
-      simp[Abbr`fml'`]
+      fs[Abbr`fml'`]
     >>
-    simp[]>>disch_then kall_tac>>
+    `interp_cclause (Dl,Dr) = {}` by
+      fs[interp_cclause_toAList]>>
+    simp[]>>
     match_mp_tac empty_clause_imp_unsatisfiable>>
     fs[])
   >>
-    strip_tac>>last_x_assum drule>>
-    `wf_clause (-h'::C)` by
-      (fs[wf_clause_def,wf_fml_def]>>
-      fs[values_def,PULL_EXISTS]>>
-      first_x_assum drule>>
-      `MEM h' (FILTER (λx. ¬MEM x C) x )` by fs[]>>
-      rw[]>>`h' ≠ 0` by metis_tac[MEM_FILTER]>>
-      intLib.ARITH_TAC)>>
-    disch_then drule>>simp[]>>
+    (last_x_assum drule>>
     simp[asymmetric_tautology_def]>>
     rw[]>>fs[]>>
     qmatch_goalsub_abbrev_tac`unsatisfiable fml'`>>
-    first_x_assum(qspec_then `fml'` mp_tac)>>
-    disch_then(qspec_then`x` mp_tac)>> impl_tac>- simp[Abbr`fml'`]>>
-    `x INSERT fml' = fml'` by
+    `(interp_cclause x) INSERT fml' = fml'` by
       (match_mp_tac ABSORPTION_RWT>>
-      fs[Abbr`fml'`,values_def]>>
+      fs[Abbr`fml'`,values_def,interp_def]>>
       metis_tac[])>>
-    simp[]>>
-    fs[Abbr`fml'`]>>
-    disch_then kall_tac>>
-    fs[UNION_INSERT_EQ]
+    pop_assum (SUBST1_TAC  o SYM)>>
+    match_mp_tac filter_unit_preserves_unsatisfiable>>
+    qexists_tac`interp_cclause C`>>rw[]
+    >-
+      simp[Abbr`fml'`]
+    >>
+      fs[interp_cclause_toAList,interp_cclause_insert_literal,Abbr`fml'`]>>
+      fs[UNION_INSERT_EQ,negate_literal_def])
+QED
+
+Theorem satisfies_clause_DIFF:
+  satisfies_clause w C ∧
+  ¬satisfies_clause w D ⇒
+  satisfies_clause w (C DIFF D)
+Proof
+  fs[satisfies_clause_def]>>
+  metis_tac[]
 QED
 
 Theorem is_AT_imp_sat_preserving:
   ∀is fml C D.
-  wf_fml fml ∧ wf_clause C ∧
   is_AT fml is C = SOME (INR D) ⇒
   ∃E.
-    D = E ++ C ∧ wf_clause D ∧
+    interp_cclause D = E ∪ interp_cclause C ∧
     ∀w.
-    satisfies w (D INSERT values fml) ⇒
-    satisfies w (C INSERT values fml)
+    satisfies w (interp_cclause D INSERT interp fml) ⇒
+    satisfies w (interp_cclause C INSERT interp fml)
 Proof
-  Induct>>fs[is_AT_def] >>
+  Induct>>fs[is_AT_def]
+  >-
+    (rw[]>>qexists_tac`{}`>>fs[])>>
   rw[]>>
   every_case_tac>>fs[]>>
-  first_x_assum drule>>
-  `wf_clause (-h'::C)` by
-    (fs[wf_clause_def,wf_fml_def]>>
-    fs[values_def,PULL_EXISTS]>>
+  pairarg_tac>>fs[]>>
+  `interp_cclause x DIFF interp_cclause C = interp_cclause (Dl,Dr)` by
+    metis_tac[delete_literals_correct]>>
+  every_case_tac>>fs[]
+  >-
+    (first_x_assum drule>>strip_tac>>
+    fs[interp_cclause_insert_literal]>>
+    qexists_tac`E ∪ {INR q}`>>
+    CONJ_ASM1_TAC>-
+      metis_tac[UNION_ASSOC,INSERT_SING_UNION]>>
+    pop_assum SUBST_ALL_TAC>>
+    qpat_x_assum`_ D = _` SUBST_ALL_TAC>>
+    rw[]>>fs[]>>
     first_x_assum drule>>
-    `MEM h' (FILTER (λx. ¬MEM x C) x )` by fs[]>>
-    rw[]>>`h' ≠ 0` by metis_tac[MEM_FILTER]>>
-    intLib.ARITH_TAC)>>
-  disch_then drule>>
-  disch_then drule>>rw[]>>
-  qexists_tac`E++[-h']`>>fs[]>>
-  rw[]>>
-  first_x_assum drule>>
-  simp[satisfies_INSERT]>>
-  Cases_on`satisfies_clause w C`>>simp[]>>
-  Cases_on`satisfies w (values fml)`>> fs[] >>
-  `satisfies_clause w x` by
-    (fs[satisfies_def,values_def]>>metis_tac[])>>
-  `satisfies_literal w h'` by
-    (fs[satisfies_clause_def]>>
-    `¬MEM l C` by metis_tac[]>>
-    `MEM l (FILTER (λx. ¬MEM x C) x)` by
-      fs[MEM_FILTER]>>
-    rfs[]>>
-    metis_tac[])>>
-  PURE_REWRITE_TAC [Once CONS_APPEND]>>
-  simp[satisfies_clause_append,satisfies_clause_def]>>
-  `h' ≠ 0` by
-    (fs[wf_clause_def]>>
-    intLib.ARITH_TAC)>>
-  metis_tac[satisfies_literal_exclusive]
+    strip_tac>>
+    fs[satisfies_INSERT]>>
+    `satisfies_clause w (interp_cclause x)` by
+      (fs[satisfies_def,interp_def,values_def]>>
+      metis_tac[])>>
+    Cases_on`satisfies_clause w (interp_cclause C)`>>fs[]>>
+    `interp_cclause x DIFF interp_cclause C = {INL q}` by
+      fs[interp_cclause_toAList]>>
+    `satisfies_clause w {INL q}` by
+      metis_tac[satisfies_clause_DIFF]>>
+     pop_assum mp_tac>> simp[satisfies_clause_def]>>
+     simp[Once (satisfies_literal_exclusive),negate_literal_def]>>
+     fs[satisfies_clause_INSERT])
+  >>
+    (first_x_assum drule>>strip_tac>>
+    fs[interp_cclause_insert_literal]>>
+    qexists_tac`E ∪ {INL q}`>>
+    CONJ_ASM1_TAC>-
+      metis_tac[UNION_ASSOC,INSERT_SING_UNION]>>
+    pop_assum SUBST_ALL_TAC>>
+    qpat_x_assum`_ D = _` SUBST_ALL_TAC>>
+    rw[]>>fs[]>>
+    first_x_assum drule>>
+    strip_tac>>
+    fs[satisfies_INSERT]>>
+    `satisfies_clause w (interp_cclause x)` by
+      (fs[satisfies_def,interp_def,values_def]>>
+      metis_tac[])>>
+    Cases_on`satisfies_clause w (interp_cclause C)`>>fs[]>>
+    `interp_cclause x DIFF interp_cclause C = {INR q}` by
+      fs[interp_cclause_toAList]>>
+    `satisfies_clause w {INR q}` by
+      metis_tac[satisfies_clause_DIFF]>>
+     pop_assum mp_tac>> simp[satisfies_clause_def]>>
+     simp[Once (satisfies_literal_exclusive),negate_literal_def]>>
+     fs[satisfies_clause_INSERT])
+QED
+
+Theorem find_exists_mem:
+  ∀ls. find_exists s ls ⇒ ∃k v. (k ∈ domain s ∧ MEM (k,v) ls)
+Proof
+  Induct>>fs[find_exists_def]>>Cases>>fs[]>>
+  rw[]>>fs[domain_lookup]>>metis_tac[]
 QED
 
 Theorem find_tauto_correct:
-  ∀ls p C.
-  find_tauto p C ls ⇒
-  ∃l. MEM l ls ∧ MEM (-l) C ∧ l ≠ -p
+  ∀C D.
+  find_tauto C D ⇒
+  ∃l. l ∈ interp_cclause C ∧ negate_literal l ∈ interp_cclause D
 Proof
-  Induct>>rw[find_tauto_def]>>metis_tac[]
+  Cases>>Cases>>rw[find_tauto_def]>>
+  drule find_exists_mem>>
+  rw[]>>fs[MEM_toAList]>>
+  fs[interp_cclause_def,domain_lookup]
+  >-
+    (qexists_tac`INL k`>>simp[negate_literal_def])
+  >>
+    qexists_tac`INR k`>>simp[negate_literal_def]
+QED
+
+Theorem interp_cclause_cclause_union:
+  interp_cclause (cclause_union C D)=
+  interp_cclause C ∪ interp_cclause D
+Proof
+  Cases_on`C`>>Cases_on`D`>>fs[cclause_union_def,interp_cclause_def]>>
+  simp[domain_union]>>
+  metis_tac[UNION_COMM,UNION_ASSOC]
 QED
 
 Theorem is_RAT_aux_imp:
   ∀iCs fml p C ik.
-  is_RAT_aux fml p C ik iCs ∧
-  wf_fml fml ∧
-  EVERY (λ(i,Ci). wf_clause Ci) iCs ∧
-  wf_clause C ⇒
-  ∀i Ci. MEM (i,Ci) iCs ∧ MEM (-p) Ci ⇒
-    asymmetric_tautology (values fml) (C ++ delete_literal (-p) Ci)
+  is_RAT_aux fml p C ik iCs ⇒
+  ∀i Ci. MEM (i,Ci) iCs ∧ has_neg_literal p Ci ⇒
+    asymmetric_tautology (interp fml) (interp_cclause C ∪ interp_cclause (delete_neg_literal p Ci))
 Proof
   Induct>>Cases>>fs[is_RAT_aux_def]>>
-  ntac 5 strip_tac >>
-  rw[]
-  >- (
-    last_x_assum kall_tac>> fs[]>>
-    every_case_tac>>fs[]
-    >-
-      (drule find_tauto_correct>>
-      rw[]>>
-      match_mp_tac (GEN_ALL tautology_asymmetric_tautology)>>
-      qexists_tac`l`>>simp[delete_literal_def,MEM_FILTER]>>
-      fs[wf_clause_def,MEM_FILTER])>>
-    match_mp_tac is_AT_imp_asymmetric_tautology>> fs[]>>
-    qexists_tac`h::t`>>fs[wf_clause_def]>>
-    fs[delete_literal_def,MEM_FILTER])
+  ntac 4 strip_tac >>
+  reverse IF_CASES_TAC>>fs[]
+  >-
+    (* 5.1 *)
+    (strip_tac>>fs[PULL_FORALL,AND_IMP_INTRO]>>
+    rw[]>>first_x_assum match_mp_tac>>fs[]>>
+    metis_tac[])
   >>
-    fs[PULL_FORALL,AND_IMP_INTRO]>>
-    first_x_assum match_mp_tac>>fs[]>>
-    every_case_tac>>fs[]>>metis_tac[]
+  TOP_CASE_TAC>>
+  TOP_CASE_TAC>-
+    (strip_tac>>first_x_assum drule>> simp[]>>
+    reverse (rw[]) >- metis_tac[]>>
+    match_mp_tac (GEN_ALL tautology_asymmetric_tautology)>>
+    drule find_tauto_correct>>
+    rw[]>>qexists_tac`l`>>simp[])
+  >>
+  (* 5.3 *)
+  reverse (rw[]>>fs[])
+  >- metis_tac[]
+  >>
+  last_x_assum kall_tac>> fs[]>>
+  drule is_AT_imp_asymmetric_tautology>>
+  metis_tac[interp_cclause_cclause_union]
+QED
+
+Theorem delete_literal_negate_literal:
+  delete_literal (negate_literal p) (interp_cclause x) = interp_cclause (delete_neg_literal p x)
+Proof
+  Cases_on`p`>>
+  Cases_on`x`>>
+  simp[delete_literal_def,delete_neg_literal_def,interp_cclause_def,EXTENSION,negate_literal_def]>>
+  rw[EQ_IMP_THM]
+QED
+
+Theorem has_literal_literal:
+  has_literal p x ⇔ p ∈ interp_cclause x
+Proof
+  Cases_on`x`>>Cases_on`p`>>simp[has_literal_def,interp_cclause_def]>>
+  simp[domain_lookup]
+QED
+
+Theorem has_neg_literal_negate_literal:
+  has_neg_literal p x ⇔ negate_literal p ∈ interp_cclause x
+Proof
+  Cases_on`x`>>Cases_on`p`>>simp[has_neg_literal_def,negate_literal_def,interp_cclause_def]>>
+  simp[domain_lookup]
 QED
 
 Theorem is_RAT_imp_resolution_asymmetric_tautology:
-  ∀fml C i0 ik.
-  wf_fml fml ∧ wf_clause C ∧
-  is_RAT fml C i0 ik ⇒
-  satisfiable (values fml) ⇒ satisfiable (C INSERT values fml)
+  ∀fml p C i0 ik.
+  is_RAT fml p C i0 ik ⇒
+  satisfiable (interp fml) ⇒ satisfiable ((interp_cclause C) INSERT interp fml)
 Proof
   rw[is_RAT_def]>>
   ntac 2 (pop_assum mp_tac)>> ntac 2 TOP_CASE_TAC>>fs[]
@@ -705,23 +914,17 @@ Proof
     (drule is_AT_imp_asymmetric_tautology>>
     rpt (disch_then drule)>>
     metis_tac[asymmetric_tautology_satisfiable]) >>
-  TOP_CASE_TAC>>fs[]>>
-  strip_tac>>
   drule is_AT_imp_sat_preserving>>
-  disch_then drule>>
-  disch_then drule>>rw[]>>
-  qmatch_asmsub_abbrev_tac`wf_clause y`>>
-  drule is_RAT_aux_imp>> simp[]>>
-  `EVERY (λ(i,Ci). wf_clause Ci) (toAList fml)` by
-    (fs[EVERY_MEM,MEM_toAList,FORALL_PROD,wf_fml_def,values_def]>>
-    metis_tac[])>>
+  rw[]>>
+  drule is_RAT_aux_imp>>
+  fs[has_literal_literal]>>
   simp[MEM_toAList]>>
   strip_tac>>
-  `resolution_asymmetric_tautology (values fml) y` by
+  `resolution_asymmetric_tautology (interp fml) (interp_cclause y)` by
     (simp[resolution_asymmetric_tautology_def]>>
-    fs[wf_clause_def]>>
-    `MEM h y` by fs[Abbr`y`]>>
-    fs[values_def,PULL_EXISTS]>>
+    DISJ2_TAC>>
+    qexists_tac`p`>>fs[interp_def,PULL_EXISTS,values_def]>>
+    fs[delete_literal_negate_literal,has_neg_literal_negate_literal]>>
     metis_tac[])>>
   drule resolution_asymmetric_tautology_satisfiable>>
   metis_tac[satisfiable_def]
@@ -729,21 +932,24 @@ QED
 
 (* Deletion preserves sat: if C is satisfiable, then deleting clauses from C keeps satisfiability *)
 Theorem delete_preserves_satisfiable:
-   satisfiable (values C) ⇒ satisfiable (values (delete n C))
+  satisfiable (interp C) ⇒ satisfiable (interp (delete n C))
 Proof
   match_mp_tac satisfiable_SUBSET>>
+  simp[interp_def]>>
+  match_mp_tac IMAGE_SUBSET>>
   metis_tac[values_delete]
 QED
 
 Theorem delete_clauses_sound:
-  ∀l fml. satisfiable (values fml) ⇒
-  satisfiable (values (delete_clauses l fml))
+  ∀l fml. satisfiable (interp fml) ⇒
+  satisfiable (interp (list_delete l fml))
 Proof
-  simp[delete_clauses_def]>>
+  simp[list_delete_def]>>
   Induct>>simp[]>>
-  metis_tac[delete_preserves_satisfiable]
+  rw[]>>metis_tac[delete_preserves_satisfiable]
 QED
 
+(*
 Theorem wf_fml_delete_clauses:
   ∀l fml.
   wf_fml fml ⇒
@@ -766,54 +972,56 @@ Proof
   drule values_insert>>
   metis_tac[]
 QED
+*)
+Theorem interp_insert:
+  interp (insert n p fml) ⊆ interp_cclause p INSERT interp fml
+Proof
+  simp[interp_def,SUBSET_DEF,PULL_EXISTS]>>
+  rw[]>>drule values_insert>>rw[]>>
+  metis_tac[]
+QED
 
 (* The main theorem *)
 Theorem check_lrat_sound:
   ∀lrat fml fml'.
-  wf_fml fml ∧
   check_lrat lrat fml = SOME fml' ⇒
-  satisfiable (values fml) ⇒ satisfiable (values fml')
+  satisfiable (interp fml) ⇒ satisfiable (interp fml')
 Proof
   Induct >> fs[check_lrat_def]>>
   Cases
   >- (
     simp[]>>
-    metis_tac[delete_clauses_sound,wf_fml_delete_clauses])
+    metis_tac[delete_clauses_sound])
   >>
   rw[]>>
   every_case_tac>>fs[]>>
-  drule wf_fml_insert>> disch_then drule>>
-  disch_then(qspec_then`n`assume_tac)>>
   first_x_assum drule>>
-  disch_then drule>>
   disch_then match_mp_tac>>
-  last_x_assum assume_tac>>
+  fs[has_literal_literal]>>
   drule is_RAT_imp_resolution_asymmetric_tautology>>
   disch_then drule>>
-  disch_then drule>>
-  disch_then drule>>
   match_mp_tac satisfiable_SUBSET>>
-  metis_tac[values_insert2]
+  metis_tac[interp_insert]
 QED
 
 Theorem check_lrat_unsat_sound:
   ∀lrat fml fml'.
-  wf_fml fml ∧
   check_lrat_unsat lrat fml ⇒
-  unsatisfiable (values fml)
+  unsatisfiable (interp fml)
 Proof
   rw[check_lrat_unsat_def]>>
   every_case_tac>>fs[MEM_MAP]>>
-  `unsatisfiable (values x)` by
+  `unsatisfiable (interp x)` by
     (match_mp_tac empty_clause_imp_unsatisfiable>>
-    fs[values_def]>>
-    metis_tac[MEM_toAList,PAIR])>>
+    Cases_on`y`>>fs[interp_def,values_def,MEM_toAList]>>
+    `interp_cclause r = {}` by
+      rw[interp_cclause_def]>>
+    metis_tac[])>>
   drule check_lrat_sound>>
-  disch_then drule>>
   metis_tac[unsatisfiable_def]
 QED
 
-(* Try on an example *)
+(* Try on an example
 val fml = rconc (EVAL ``insert 1 [ 1;  2; -3] (
   insert 2 [-1; -2;  3] (
   insert 3 [ 2;  3; -4] (
@@ -821,7 +1029,7 @@ val fml = rconc (EVAL ``insert 1 [ 1;  2; -3] (
   insert 5 [-1; -3; -4] (
   insert 6 [ 1;  3;  4] (
   insert 7 [-1;  2;  4] (
-  insert 8 [ (1:int); -2; -4] LN)))))))``)
+  insert 8 [ (1:int); -2; -4] LN))))))) :ccnf``)
 
 val lrat =
 ``[
@@ -835,5 +1043,5 @@ val lrat =
 
   (* result contains the empty clause *)
 val res = EVAL``check_lrat_unsat ^(lrat) ^(fml)``
-
+ *)
 val _ = export_theory ();
